\documentclass[12pt]{article}
\usepackage{amsmath,amssymb,amsthm,verbatim}

%*****************************************************************
%			Dimensions

\setlength{\textheight}{9in}
\setlength{\textwidth}{6.5in}
\setlength{\oddsidemargin}{0in}
\setlength{\evensidemargin}{0in}
\setlength{\hoffset}{0in}
\setlength{\voffset}{-1in}
\setlength{\footskip}{.5in}
\setlength{\parskip}{10pt}
\setlength{\parindent}{0pt}

\pagestyle{empty}

%*****************************************************************

%****************************************************************
                

\begin{document}

\begin{flushright}
\begin{tabular}{l}
Christopher David Miller \\  % Enter your name here
FSMAT 201 \\  % The current class. You can change this if you want to use this for other classes.
Problem 3.1 \\  % Replace x with the appropriate problem number
Version 1 \\ %If this is the first time you've submitted this solution, let n=1. If this is a first resubmission, let n=2, etc. 
\end{tabular}
\end{flushright}
\vspace{20pt}  % Just adding some extra vertical space.

% Now write out the statement of the problem, followed by your solution. 

\textbf{3.1} \\  % Replace x with the appropriate problem number
Let $z = a + bi$ and $w = c + di $. Prove that $\overline{zw} = \overline{z} \cdot \overline{w}$.


To prove this statement we need to introduce the definition of the conjugate of a complex number. Let $q$ be a complex number, in other words $q = c + di$ where $c$ and $d$ are real numbers. The conjugate of $q$, denoted by $\overline{q}$, is defined by $$\overline{q}= c - di.$$
Now we have enough definitions to finish our proof.
\begin{proof}
  
  Let $z = a + bi$ and $w = c + di $. In order to show that  $\overline{zw} = \overline{z} \cdot \overline{w}$. We need to calculate $\overline{zw}$ and $\overline{z} \cdot \overline{w}$ .
  \begin{equation*}
    \begin{aligned}[c]
      \overline{zw} &= \overline{(a+bi)(c+di)} \\ 
       &= \overline{ac+adi+bci-bd}\\
       &= \overline{(ac-bd)+i(ad+bc)}\\
       &= (ac-bd)-i(ad+bc)  
    \end{aligned}
    \begin{aligned}[c]
      \overline{z} \cdot \overline{w} &= \overline{(a+bi)} \cdot \overline{(c+di)} \\ 
       &= (a-bi) \cdot (c-di)\\
       &= ac -adi-bci-bd\\
       &= (ac-bd)-i(ad+bc)  
    \end{aligned}
  \end{equation*}
  We have shown that $\overline{zw} = \overline{z} \cdot \overline{w}$
    
      
      

    
\end{proof}
\newpage
\begin{flushright}
  \begin{tabular}{l}
  Christopher David Miller \\  % Enter your name here
  FSMAT 201 \\  % The current class. You can change this if you want to use this for other classes.
  Problem 3.2 \\  % Replace x with the appropriate problem number
  Version 1 \\ %If this is the first time you've submitted this solution, let n=1. If this is a first resubmission, let n=2, etc. 
  \end{tabular}
  \end{flushright}
  \vspace{20pt}  % Just adding some extra vertical space.
  
  % Now write out the statement of the problem, followed by your solution. 
  
  \textbf{3.2} \\  % Replace x with the appropriate problem number
  Let $z = a + bi$ and $w = c + di $. Prove that $\lvert zw \rvert = \lvert z \rvert \cdot \lvert w \rvert$.
  
  
  To prove this statement we need to introduce the definition of the modulus of a complex number. Let $q$ be a complex number, in other words $q = c + di$ where $c$ and $d$ are real numbers. The modulus of $q$, denoted by $\lvert q \rvert$, is defined by $$\lvert q \rvert= \sqrt{c^2 + d^2}$$
  Now we have enough definitions to finish our proof.
  \begin{proof}
    
    Let $z = a + bi$ and $w = c + di $. In order to show that  $\lvert zw \rvert = \lvert z \rvert \cdot \lvert w \rvert$. We need to calculate $\lvert zw \rvert$ and $\lvert z \rvert \cdot \lvert w \rvert.$
    \begin{equation*}
      \begin{aligned}[c]
        \lvert z \rvert \cdot \lvert w \rvert &= \sqrt{a^2 + b^2} \cdot \sqrt{c^2 + d^2} \\ 
         &= \sqrt{(a^2 + b^2)(c^2 + d^2)}\\
         &= \sqrt{a^2c^2 + a^2d^2 + b^2c^2+b^2d^2}
      \end{aligned}
      \begin{aligned}[c]
        \lvert zw \rvert &= \overline{(a+bi)} \cdot \overline{(c+di)} \\ 
         &= (a-bi) \cdot (c-di)\\
         &= ac -adi-bci-bd\\
         &= (ac-bd)-i(ad+bc)  
      \end{aligned}
    \end{equation*}
    We have shown that $\overline{zw} = \overline{z} \cdot \overline{w}$
      
        
        
  
      
  \end{proof}






\end{document}











